src/coq/Utils/ITreeRaise.v
@@ -12,10 +12,22 @@ From ITree Require Import
      ITree.
 
 From Vellvm Require Import 
-     Semantics.LLVMEvents.
+     Semantics.LLVMEvents
+     Utils.MonadExcLaws.
 
+Section Laws.
+  Variable E : Type -> Type.
+  Variable MSG : Type.
 
-Section Itree.
+  Class RaiseBindItree :=
+    { rbi_raise : forall {X}, MSG -> itree E X;
+      rbi_raise_bind :
+      forall A B (f : A -> itree E B) (x : MSG),
+        bind (rbi_raise x) f ≈ rbi_raise x      
+    }.
+End Laws.
+
+Section Failure.
   Variable E : Type -> Type.
   Context {FAIL : FailureE -< E}.
 
@@ -32,4 +44,57 @@ Section Itree.
     intros u1 u2 H.
     destruct u1.
   Qed.
-End Itree.
+
+  Global Instance RaiseBindItree_Fail : RaiseBindItree E string :=
+    { rbi_raise := fun X => raise;
+      rbi_raise_bind := raise_bind_itree
+    }.
+End Failure.
+
+Section OOM.
+  Variable E : Type -> Type.
+  Context {OOM : OOME -< E}.
+
+  Lemma raiseOOM_bind_itree :
+    forall A B (f : A -> itree E B) x,
+      bind (raiseOOM x) f ≈ raiseOOM x.
+  Proof.
+    intros A B f x.
+    unfold raiseOOM.
+    cbn.
+    rewrite bind_bind.
+    eapply eutt_clo_bind.
+    reflexivity.
+    intros u1 u2 H.
+    destruct u1.
+  Qed.
+
+  Global Instance RaiseBindItree_OOM : RaiseBindItree E string :=
+    { rbi_raise := fun X => raiseOOM;
+      rbi_raise_bind := raiseOOM_bind_itree
+    }.
+End OOM.
+
+Section UB.
+  Variable E : Type -> Type.
+  Context {UB : UBE -< E}.
+
+  Lemma raiseUB_bind_itree :
+    forall A B (f : A -> itree E B) x,
+      bind (raiseUB x) f ≈ raiseUB x.
+  Proof.
+    intros A B f x.
+    unfold raiseUB.
+    cbn.
+    rewrite bind_bind.
+    eapply eutt_clo_bind.
+    reflexivity.
+    intros u1 u2 H.
+    destruct u1.
+  Qed.
+
+  Global Instance RaiseBindItree_UB : RaiseBindItree E string :=
+    { rbi_raise := fun X => raiseUB;
+      rbi_raise_bind := raiseUB_bind_itree
+    }.
+End UB.
