src/coq/Handlers/FiniteMemoryTheory.v
@@ -3376,3 +3376,5 @@ End MEMORY_THEORY.
 Module Make (LP : LLVMParams) (Events : LLVM_INTERACTIONS LP.ADDR LP.IP LP.SIZEOF) (MP : MemoryParams LP Events) (SP : SerializationParams LP Events MP) (Mem : FinMemory LP Events MP) <: MEMORY_THEORY LP Events MP SP Mem.
 Include MEMORY_THEORY LP Events MP SP Mem.
 End Make.
+
+
